proved some properties about sin and cosine

IRLemmasAsCR.v
@@ -8,22 +8,160 @@ Require Export MathClasses.interfaces.canonical_names.
 Require Export MathClasses.misc.decision.
 Require Export MathClasses.interfaces.abstract_algebra.
 
-Instance castCRIR : Cast CR IR := CRasIR.
 
-Instance inj_CRasIR : Injective  CRasIR.
+Instance Injective_instance_CRasIR : Injective  CRasIR.
   constructor.
 - intros ? ? Heq. apply (fun_strext_imp_wd _ _ IRasCR) in Heq;
     [ | apply R_morphism.map_strext].
-  rewrite CRasIRasCR_id in Heq.
-  rewrite CRasIRasCR_id in Heq.
+  repeat( rewrite CRasIRasCR_id in Heq).
   exact Heq.
-- constructor; eauto 2 with *.
+- constructor;eauto 2 with *.
   exact CRasIR_wd.
 Qed.
 
+Instance Injective_instance_IRasCR : Injective  IRasCR.
+  constructor.
+- intros ? ? Heq. apply (fun_strext_imp_wd _ _ CRasIR) in Heq;
+    [ | apply R_morphism.map_strext].
+  repeat (rewrite IRasCRasIR_id in Heq).
+  exact Heq.
+- constructor; try apply st_isSetoid.
+  exact IRasCR_wd.
+Qed.
 
+Lemma CRasIR_inv :  forall x, (CRasIR (- x) = [--] (CRasIR x))%CR.
+Proof.
+  intros. apply (injective IRasCR).
+  rewrite IR_opp_as_CR.
+  rewrite CRasIRasCR_id, CRasIRasCR_id.
+  reflexivity.
+Qed.
 
+  
+Require Export CoRN.reals.fast.CRArith.
 
+Lemma sr_mult_associative `{SemiRing R} (x y z : R) : x * (y * z) = x * y * z.
+Proof. apply sg_ass, _. Qed.
 
+Lemma inject_Q_CR_one  : (inject_Q_CR (1#1) [=] 1)%CR.
+ring.
+Qed.
 
+Lemma inject_Q_CR_two  : (inject_Q_CR (2#1) = 2)%CR.
+  rewrite <- inject_Q_CR_one.
+  destruct CR_Q_ring_morphism.
+  idtac. unfold plus, CRplus. rewrite <- morph_add; eauto.
+Qed.
 
+Definition QCRM := CR_Q_ring_morphism.
+
+Lemma CR_Cos_HalfPi : (cos (CRpi * ' (1 # 2)) = 0 )%CR.
+Proof.
+  pose proof (Pi.Cos_HalfPi) as Hc.
+  apply IRasCR_wd in Hc.
+  autorewrite with IRtoCR in Hc.
+  rewrite <- Hc.
+  apply sm_proper.
+  apply (right_cancellation mult 2).
+  match goal with 
+  [ |- ?l = _] => remember l as ll
+  end.
+  rewrite <- IR_One_as_CR.
+  unfold plus. unfold CRplus.
+  rewrite <- IR_plus_as_CR.
+  rewrite <- IR_mult_as_CR.
+  subst.
+  apply (injective CRasIR).
+  rewrite IRasCRasIR_id.
+  rewrite one_plus_one.
+  rewrite div_1.
+  apply (injective IRasCR).
+  rewrite CRasIRasCR_id.
+  rewrite CRpi_correct.
+  fold (mult).
+  rewrite <- sr_mult_associative.
+  match goal with 
+  [ |- ?l = _] => remember l as ll
+  end.
+  assert (CRpi [=] CRpi * 1)%CR as Hr by ring.
+  rewrite Hr.
+  subst ll.
+  fold (mult).
+  simpl. apply sg_op_proper;[reflexivity|].
+  rewrite <- inject_Q_CR_two.
+  rewrite <- (morph_mul QCRM).
+  apply (morph_eq QCRM).
+  reflexivity.
+Qed.
+
+Lemma CRCos_inv : forall x, (cos (-x) = cos x )%CR.
+Proof.
+  intros. rewrite <- cos_correct_CR, <- cos_correct_CR.
+  apply IRasCR_wd.
+  rewrite <- SinCos.Cos_inv.
+  apply SinCos.Cos_wd.
+  
+  pose proof (Pi.Cos_HalfPi) as Hc.
+  apply IRasCR_wd in Hc.
+  autorewrite with IRtoCR in Hc.
+  rewrite <-  CRasIR_inv.
+  apply CRasIR_wd.
+  ring.
+Qed.
+
+Lemma CR_Sin_HalfPi : (sin (CRpi * ' (1 # 2)) = 1 )%CR.
+Proof.
+  pose proof (Pi.Sin_HalfPi) as Hc.
+  apply IRasCR_wd in Hc.
+  autorewrite with IRtoCR in Hc.
+  rewrite <- Hc.
+  apply sm_proper.
+  apply (right_cancellation mult 2).
+  match goal with 
+  [ |- ?l = _] => remember l as ll
+  end.
+  rewrite <- IR_One_as_CR.
+  unfold plus. unfold CRplus.
+  rewrite <- IR_plus_as_CR.
+  rewrite <- IR_mult_as_CR.
+  subst.
+  apply (injective CRasIR).
+  rewrite IRasCRasIR_id.
+  rewrite one_plus_one.
+  rewrite div_1.
+  apply (injective IRasCR).
+  rewrite CRasIRasCR_id.
+  rewrite CRpi_correct.
+  fold (mult).
+  rewrite <- sr_mult_associative.
+  match goal with 
+  [ |- ?l = _] => remember l as ll
+  end.
+  assert (CRpi [=] CRpi * 1)%CR as Hr by ring.
+  rewrite Hr.
+  subst ll.
+  fold (mult).
+  simpl. apply sg_op_proper;[reflexivity|].
+  rewrite <- inject_Q_CR_two.
+  rewrite <- (morph_mul QCRM).
+  apply (morph_eq QCRM).
+  reflexivity.
+Qed.
+
+Lemma CRSin_inv : forall x, (sin (-x) = - sin x )%CR.
+Proof.
+  intros. rewrite <- sin_correct_CR, <- sin_correct_CR.
+  rewrite <- IR_opp_as_CR.
+  apply IRasCR_wd.
+  rewrite <- SinCos.Sin_inv.
+  apply SinCos.Sin_wd.
+  
+  pose proof (Pi.Cos_HalfPi) as Hc.
+  apply IRasCR_wd in Hc.
+  autorewrite with IRtoCR in Hc.
+  rewrite <-  CRasIR_inv.
+  apply CRasIR_wd.
+  ring.
+Qed.
+
+(*Instance castCRIR : Cast CR IR := CRasIR. *)
