CartCR.v
@@ -30,6 +30,40 @@ Definition Cart2Polar (cart :Cart2D Q) : Polar2D CR :=
   {|rad := polarRad cart 
   ; θ := polarTheta cart |}.
 
+Require Export CoRN.util.Extract.
+
+(** Time Eval vm_compute in answer 10 ((4*(polarTheta {|X:=1; Y:=1|}))).
+  = 31415926535%Z
+     : Z
+  Finished transaction in 0. secs (0.u,0.s)
+
+  Time Eval vm_compute in answer 10 ((4*(polarTheta {|X:=1; Y:=1|}))).
+  = 31415926535%Z
+     = (-31415926536)%Z
+     : Z
+  Finished transaction in 0. secs (0.0160000000005u,0.s)
+
+  Time Eval vm_compute in answer 10 ((4*(polarTheta {|X:=1; Y:=1|}))).
+  = 31415926535%Z
+     = (-31415926536)%Z
+     : Z
+  Finished transaction in 0. secs (0.0160000000005u,0.s)
+
+  Time Eval vm_compute in answer 10 
+    (((polarTheta {|X:=-1; Y:=-1|})*(cast Q CR (4#5)))).
+  
+   = 31415926535%Z
+     : Z
+  Finished transaction in 0. secs (0.0150000000003u,0.s)
+
+  Time Eval vm_compute in answer 10 
+      (((polarTheta {|X:=-1; Y:=1|})*(cast Q CR (4#3)))).
+     = 31415926535%Z
+     : Z
+  Finished transaction in 0. secs (0.0160000000005u,0.s)    
+*)
+
+
 Definition Polar2Cart (pol : Polar2D CR) : Cart2D CR :=
   {|X := (rad pol) * (cos (θ pol)) 
   ; Y := (rad pol) * (sin (θ pol)) |}.
@@ -39,6 +73,8 @@ Instance castCart `{Cast A B} : Cast (Cart2D A) (Cart2D B) :=
 
 Instance EquivCart  `{Equiv A} : Equiv (Cart2D A) :=
 fun ca cb => (X ca = X cb /\ Y ca = Y cb).
+
+Require Export IRLemmasAsCR.
 
 
 (** lets first port lemmas about IR sin cos
@@ -52,4 +88,4 @@ Proof.
   unfold polarTheta. simpl.
   destruct (decide (cx = 0)) as [Hcx0 | Hcx0].
 - split; simpl.
-Abort.
+  + 
